formalization/ParallelReduction.v
@@ -4,6 +4,9 @@ From FD Require Import FreeVars.
 From FD Require Import Renaming.
 From FD Require Import FreeVars.
 From FD Require Import StructCong.
+From FD Require Import Contexts.
+From FD Require Import Typing.
+From FD Require Import Preservation.
 From FD Require Import ConfluenceDefs.
 From FD Require Import DirectedCong.
 From FD Require Import AxCutCtx.
@@ -171,7 +174,7 @@ Proof.
   - right; auto.
 Qed.
 
-(* ↠* ∪ ▶ *)
+(* ↠* ⊂ ▶ *)
 Corollary clos_trans_par_red_in_multi_step_red :
   forall P Q, clos_trans process par_reduction P Q -> P ▶ Q.
 Proof.
@@ -186,4 +189,1106 @@ Proof.
   intros; split.
   + apply clos_trans_par_red_in_multi_step_red.
   + apply multi_step_red_in_clos_trans_par_red.
+Qed.
+
+(******************************************************************************)
+(* Parallel Reductions Preserve Typing                                        *)
+(******************************************************************************)
+Lemma par_red_preserves_typing :
+  forall Γ P Q, Γ ⊢ P :# -> P ↠ Q -> Γ ⊢ Q :#.
+Proof.
+  intros.
+  apply par_reduction_in_reduces_or_struct_cong in H0.
+  destruct H0.
+  + eapply preservation; eauto.
+  + eapply struct_cong_preserves_typing; eauto. apply c_comm; auto.
+Qed.
+
+Lemma directed_cong_preserves_typing :
+  forall Γ P Q, Γ ⊢ P :# -> P ⇛ Q -> Γ ⊢ Q :#.
+Proof.
+  intros. apply directed_cong_in_struct_cong in H0.
+  apply ((proj1 struct_cong_preserves_typing) _ _ H0) in H; auto.
+Qed.
+
+(******************************************************************************)
+(* Auxiliary Lemmata for Confluence                                           *)
+(******************************************************************************)
+Lemma link_directed_cong_equiv_red_commute :
+  forall ml mr P Q, (link ml mr) ⇛ P -> (link ml mr) ⊵ Q ->
+    exists R, P ⊵ R /\ Q ⇛ R.
+Proof.
+  intros. inversion H; inversion H0; subst;
+  try match goal with
+  | [ H1 : (prefix (send _ _))  !⇛ _,
+      H2 : (prefix (receive _)) !⇛ _
+      |- _ ] =>
+    apply directed_cong_inversion_prefix in H1; destruct H1 as [? [? H1']];
+    apply directed_cong_inversion_prefix in H2; destruct H2 as [? [? H2']];
+    apply directed_cong_inversion_send in H1'; destruct H1' as [? [? [? [? ?]]]];
+    apply directed_cong_inversion_receive in H2'; destruct H2' as [? [? ?]];
+    subst; eexists; split; 
+    [ try eapply rp_tensor_par_1; try eapply rp_tensor_par_2; auto
+    | apply dc_cong_cut; auto; apply dc_cong_cut; auto;
+      apply directed_cong_invariant_under_renaming; try apply swap01_is_bijective;
+      apply directed_cong_invariant_under_upshifting; auto ]
+  | [ H1 : (prefix (choose_left _)) !⇛ _,
+      H2 : (prefix (offer_choice _ _)) !⇛ _
+      |- _ ] =>
+    apply directed_cong_inversion_prefix in H1; destruct H1 as [? [? H1']];
+    apply directed_cong_inversion_prefix in H2; destruct H2 as [? [? H2']];
+    apply directed_cong_inversion_choosel in H1'; destruct H1' as [? [? ?]];
+    apply directed_cong_inversion_choice in H2'; destruct H2' as [? [? [? [? ?]]]];
+    subst; eexists; split; 
+    [ try eapply rp_plus_with_l1; try eapply rp_plus_with_l2; auto
+    | apply dc_cong_cut; auto; apply dc_cong_cut; auto;
+      apply directed_cong_invariant_under_renaming; try apply swap01_is_bijective;
+      apply directed_cong_invariant_under_upshifting; auto ]
+  | [ H1 : (prefix (choose_right _)) !⇛ _,
+      H2 : (prefix (offer_choice _ _)) !⇛ _
+      |- _ ] =>
+    apply directed_cong_inversion_prefix in H1; destruct H1 as [? [? H1']];
+    apply directed_cong_inversion_prefix in H2; destruct H2 as [? [? H2']];
+    apply directed_cong_inversion_chooser in H1'; destruct H1' as [? [? ?]];
+    apply directed_cong_inversion_choice in H2'; destruct H2' as [? [? [? [? ?]]]];
+    subst; eexists; split; 
+    [ try eapply rp_plus_with_r1; try eapply rp_plus_with_r2; auto
+    | apply dc_cong_cut; auto; apply dc_cong_cut; auto;
+      apply directed_cong_invariant_under_renaming; try apply swap01_is_bijective;
+      apply directed_cong_invariant_under_upshifting; auto ]
+  | [ H1 : (prefix close) !⇛ _,
+      H2 : (prefix (wait _)) !⇛ _
+      |- _ ] =>
+    apply directed_cong_inversion_prefix in H1; destruct H1 as [? [? H1']];
+    apply directed_cong_inversion_prefix in H2; destruct H2 as [? [? H2']];
+    apply directed_cong_inversion_close in H1';
+    apply directed_cong_inversion_wait in H2'; destruct H2' as [? [? ?]];
+    subst; eexists; split; [ try eapply rp_one_bot1; try eapply rp_one_bot2; eauto | auto ]
+  end.
+  + eexists. split. apply rp_refl. apply dc_cong_link; auto.
+  + inversion H; subst.
+    - eexists. split. apply rp_refl. econstructor; auto.
+    - eexists. split. apply rp_refl. apply dc_link; auto.
+Qed.
+
+(* ⊵ is invariant under arbitrary upshift of swap01 ***************************)
+(* facts and helpers about substitution *)
+Definition swap_subst (σ : substitution) (i j : nat) : substitution :=
+  fun x => if (Nat.eqb x i) then σ j else
+            if (Nat.eqb x j) then σ i else σ x.
+
+Lemma up_subst_distributes_over_swap_subst :
+  forall r σ i j, bijective r ->
+    forall x,
+      up_subst (fun x => rename_message ((swap_subst σ i j) x) r) x
+        = (fun x => rename_message (swap_subst (up_subst σ) (S i) (S j) x) (up_ren r)) x.
+Proof.
+  intros. destruct x; simpl; auto.
+  unfold swap_subst.
+  destruct (Nat.eqb x i) eqn:E1.
+  + apply PeanoNat.Nat.eqb_eq in E1. assert ((S x) = (S i)) by lia.
+    apply PeanoNat.Nat.eqb_eq in H0. rewrite H0. simpl.
+    unfold upM.
+    rewrite (proj1 (proj2 ren_up_up_ren_commute)); auto.
+    intros. exfalso; lia.
+  + apply PeanoNat.Nat.eqb_neq in E1. assert ((S x) <> (S i)) by lia.
+    apply PeanoNat.Nat.eqb_neq in H0. rewrite H0. simpl.
+    destruct (Nat.eqb x j) eqn:E2.
+    - unfold upM. rewrite (proj1 (proj2 ren_up_up_ren_commute)); auto. intros; exfalso; lia.
+    - unfold upM. rewrite (proj1 (proj2 ren_up_up_ren_commute)); auto. intros; exfalso; lia.
+Qed.
+
+Lemma up_subst_distributes_over_swap_subst2 :
+  forall r σ i j, bijective r ->
+    forall x,
+      up_subst (up_subst (fun x => rename_message ((swap_subst σ i j) x) r)) x
+        = (fun x => rename_message (swap_subst (up_subst (up_subst σ)) (S (S i)) (S (S j)) x) (up_ren (up_ren r))) x.
+Proof.
+  intros. destruct x; simpl; auto.
+  unfold swap_subst.
+  destruct (Nat.eqb (S x) (S (S i))) eqn:E1.
+  + simpl. apply PeanoNat.Nat.eqb_eq in E1. inversion E1; subst; simpl.
+    unfold upM. rewrite (proj1 (proj2 ren_up_up_ren_commute)).
+    - rewrite PeanoNat.Nat.eqb_refl.
+      f_equal. rewrite (proj1 (proj2 ren_up_up_ren_commute)); auto.
+      intros. exfalso; lia.
+    - apply shift_preserves_bijection; auto.
+    - intros; exfalso; lia.
+  + apply PeanoNat.Nat.eqb_neq in E1. destruct x; simpl; auto.
+    assert (x <> i) by lia. apply PeanoNat.Nat.eqb_neq in H0. rewrite H0.
+    destruct (Nat.eqb x j) eqn:E2.
+    - unfold upM. rewrite (proj1 (proj2 ren_up_up_ren_commute)).
+      * f_equal. rewrite (proj1 (proj2 ren_up_up_ren_commute)); auto. intros; exfalso; lia.
+      * apply shift_preserves_bijection; auto.
+      * intros; exfalso; lia.
+    - unfold upM. rewrite (proj1 (proj2 ren_up_up_ren_commute)).
+      * f_equal. rewrite (proj1 (proj2 ren_up_up_ren_commute)); auto. intros; exfalso; lia.
+      * apply shift_preserves_bijection; auto.
+      * intros; exfalso; lia.
+Qed.
+
+Lemma subst_extensional :
+  (forall P, forall σ1 σ2, (forall x, σ1 x = σ2 x) ->
+    subst_process P σ1 = subst_process P σ2) /\
+  (forall M, forall σ1 σ2, (forall x, σ1 x = σ2 x) ->
+    subst_message M σ1 = subst_message M σ2) /\
+  (forall s, forall σ1 σ2, (forall x, σ1 x = σ2 x) ->
+    subst_statement s σ1 = subst_statement s σ2).
+Proof.
+  apply syntax_ind; intros; simpl; auto.
+  try (now (try rewrite (H σ1 σ2); auto; try rewrite (H0 σ1 σ2); auto)).
+  + rewrite (H _ (up_subst σ2)); try rewrite (H0 _ (up_subst σ2)); auto;
+    intros [|]; auto; simpl; rewrite H1; auto.
+  + rewrite (H _ (up_subst σ2)); try rewrite (H0 _ σ2); auto;
+    intros [|]; auto; simpl; rewrite H1; auto.
+  + rewrite (H _ σ2); auto.
+  + rewrite (H _ (up_subst σ2)); auto; intros [|]; auto; simpl; rewrite H0; auto.
+  + rewrite (H _ (up_subst σ2)); auto; intros [|]; auto; simpl; rewrite H0; auto.
+  + rewrite (H _ (up_subst σ2)); try rewrite (H0 _ (up_subst σ2)); auto;
+    intros [|]; auto; simpl; rewrite H1; auto.
+  + rewrite (H _ (up_subst σ2)); try rewrite (H0 _ (up_subst σ2)); auto;
+    intros [|]; auto; simpl; rewrite H1; auto.
+  + rewrite (H _ (up_subst (up_subst σ2))); auto; intros [|[|]]; auto;
+    simpl; rewrite H0; auto.
+  + rewrite (H _ σ2); auto.
+Qed.
+
+Lemma up_ren_n_swap_n :
+  forall n, up_ren_n n swap01 n = S n.
+Proof.
+  induction n; auto. simpl. rewrite IHn; auto.
+Qed.
+
+Lemma up_ren_n_swap_Sn :
+  forall n, up_ren_n n swap01 (S n) = n.
+Proof.
+  induction n; auto. simpl. rewrite IHn; auto.
+Qed.
+
+Lemma up_ren_n_swap_not_nSn :
+  forall n j, n <> j -> S n <> j -> up_ren_n n swap01 j = j.
+Proof.
+  induction n; intros; simpl.
+  + destruct j; try (exfalso; lia); destruct j; try (exfalso; lia).
+    auto.
+  + destruct j; auto; simpl.
+    assert (n <> j) by lia.
+    assert (S n <> j) by lia.
+    rewrite IHn; auto.
+Qed.
+
+Lemma up_ren_swap_over_subst :
+  (
+    forall P, forall σ j,
+      rename_process (subst_process P σ) (up_ren_n j swap01) =
+      subst_process (rename_process P (up_ren_n (S j) swap01))
+                    (fun x => rename_message (swap_subst σ (S j) (S (S j)) x) (up_ren_n j swap01))
+  ) /\
+  (
+    forall M, forall σ j,
+      rename_message (subst_message M σ) (up_ren_n j swap01) =
+      subst_message (rename_message M (up_ren_n (S j) swap01))
+                    (fun x => rename_message (swap_subst σ (S j) (S (S j)) x) (up_ren_n j swap01))
+  ) /\
+  (
+    forall s, forall σ j,
+      rename_statement (subst_statement s σ) (up_ren_n j swap01) =
+      subst_statement (rename_statement s (up_ren_n (S j) swap01))
+                    (fun x => rename_message (swap_subst σ (S j) (S (S j)) x) (up_ren_n j swap01))
+  ).
+Proof.
+  apply syntax_ind; intros; simpl;
+  try (now (try rewrite H; try rewrite H0; auto)).
+  + replace (up_ren (up_ren_n j swap01)) with (up_ren_n (S j) swap01) by auto.
+    rewrite H. rewrite H0. f_equal.
+    - apply (proj1 subst_extensional). intro x.
+      rewrite up_subst_distributes_over_swap_subst; auto.
+      apply up_ren_n_preserves_bijection; apply swap01_is_bijective.
+    - apply (proj1 subst_extensional). intro x.
+      rewrite up_subst_distributes_over_swap_subst; auto.
+      apply up_ren_n_preserves_bijection; apply swap01_is_bijective.
+  + replace (up_ren (up_ren_n j swap01)) with (up_ren_n (S j) swap01) by auto.
+    rewrite H0. f_equal. rewrite H. apply (proj1 subst_extensional). intro x.
+    rewrite up_subst_distributes_over_swap_subst; auto.
+    apply up_ren_n_preserves_bijection; apply swap01_is_bijective.
+  + replace (up_ren (up_ren_n j swap01)) with (up_ren_n (S j) swap01) by auto.
+    f_equal.
+    destruct (PeanoNat.Nat.eq_dec (S j) n).
+    - subst. rewrite up_ren_n_swap_n.
+      unfold swap_subst. assert (S (S j) <> S j) by lia.
+      apply PeanoNat.Nat.eqb_neq in H; rewrite H.
+      rewrite PeanoNat.Nat.eqb_refl. auto.
+    - destruct (PeanoNat.Nat.eq_dec (S (S j)) n).
+      * subst. rewrite up_ren_n_swap_Sn. unfold swap_subst.
+        rewrite PeanoNat.Nat.eqb_refl. auto.
+      * rewrite up_ren_n_swap_not_nSn; auto.
+        unfold swap_subst. assert (n <> S j) by lia. assert (n <> S (S j)) by lia.
+        apply PeanoNat.Nat.eqb_neq in H, H0.
+        rewrite H. rewrite H0. auto.
+  + replace (up_ren (up_ren_n j swap01)) with (up_ren_n (S j) swap01) by auto.
+    rewrite H. f_equal. apply (proj1 subst_extensional). intro x.
+    rewrite up_subst_distributes_over_swap_subst; auto.
+    apply up_ren_n_preserves_bijection; apply swap01_is_bijective.
+  + replace (up_ren (up_ren_n j swap01)) with (up_ren_n (S j) swap01) by auto.
+    rewrite H. f_equal. apply (proj1 subst_extensional). intro x.
+    rewrite up_subst_distributes_over_swap_subst; auto.
+    apply up_ren_n_preserves_bijection; apply swap01_is_bijective.
+  + replace (up_ren (up_ren_n j swap01)) with (up_ren_n (S j) swap01) by auto.
+    rewrite H. rewrite H0. f_equal.
+    - apply (proj1 subst_extensional). intro x.
+      rewrite up_subst_distributes_over_swap_subst; auto.
+      apply up_ren_n_preserves_bijection; apply swap01_is_bijective.
+    - apply (proj1 subst_extensional). intro x.
+      rewrite up_subst_distributes_over_swap_subst; auto.
+      apply up_ren_n_preserves_bijection; apply swap01_is_bijective.
+  + replace (up_ren (up_ren_n j swap01)) with (up_ren_n (S j) swap01) by auto.
+    rewrite H. rewrite H0. f_equal.
+    - apply (proj1 subst_extensional). intro x.
+      rewrite up_subst_distributes_over_swap_subst; auto.
+      apply up_ren_n_preserves_bijection; apply swap01_is_bijective.
+    - apply (proj1 subst_extensional). intro x.
+      rewrite up_subst_distributes_over_swap_subst; auto.
+      apply up_ren_n_preserves_bijection; apply swap01_is_bijective.
+  + f_equal.
+    replace (up_ren (up_ren (up_ren_n j swap01))) with (up_ren_n (S (S j)) swap01) by auto.
+    rewrite H. apply subst_extensional. intro x.
+    rewrite up_subst_distributes_over_swap_subst2; auto.
+    apply up_ren_n_preserves_bijection; apply swap01_is_bijective.
+Qed.
+
+Lemma up_ren_swap_over_reduce_axcut' :
+  forall n E M P j,
+    n = length_axcut_ctx E ->
+    well_formed_axcut_ctx 0 E ->
+    ~ (occurs_free_message n M) ->
+    rename_process (reduce_axcut E M P) (up_ren_n j swap01) =
+    reduce_axcut
+      (rename_axcut_ctx E (up_ren_n (S j) swap01))
+      (rename_message M (up_ren_n (length_axcut_ctx E + (S j)) swap01))
+      (rename_process P (up_ren_n (S j) swap01)).
+Proof.
+  intro n.
+  induction n; intros; simpl;
+  destruct E; simpl in H; try congruence; simpl.
+  + repeat rewrite reduce_axcut_equation_1.
+    replace (up_ren (up_ren_n j swap01)) with (up_ren_n (S j) swap01) by auto.
+    rewrite (proj1 up_ren_swap_over_subst).
+    apply subst_extensional. intros x.
+    destruct (PeanoNat.Nat.eq_dec (S j) x).
+    - subst. simpl. unfold swap_subst. rewrite PeanoNat.Nat.eqb_refl.
+      simpl. rewrite up_ren_n_swap_Sn. auto.
+    - unfold swap_subst. assert (x <> S j) by lia.
+      apply PeanoNat.Nat.eqb_neq in H2; rewrite H2.
+      destruct (Nat.eqb x (S (S j))) eqn:E.
+      * simpl. rewrite up_ren_n_swap_n.
+        apply PeanoNat.Nat.eqb_eq in E; subst. simpl. auto.
+      * simpl. destruct x; simpl.
+        ** unfold downM. rewrite (proj1 (proj2 down_ren_up_ren_commute)); auto.
+           -- apply up_ren_n_preserves_bijection; apply swap01_is_bijective.
+           -- intros; exfalso; lia.
+        ** rewrite up_ren_n_swap_not_nSn; auto. apply PeanoNat.Nat.eqb_neq in E; lia.
+  + repeat rewrite reduce_axcut_equation_2.
+    replace (up_ren (up_ren_n j swap01)) with (up_ren_n (S j) swap01) by auto.
+    rewrite (proj1 up_ren_swap_over_subst).
+    apply subst_extensional. intros x.
+    destruct (PeanoNat.Nat.eq_dec (S j) x).
+    - subst. simpl. unfold swap_subst. rewrite PeanoNat.Nat.eqb_refl.
+      simpl. rewrite up_ren_n_swap_Sn. auto.
+    - unfold swap_subst. assert (x <> S j) by lia.
+      apply PeanoNat.Nat.eqb_neq in H2; rewrite H2.
+      destruct (Nat.eqb x (S (S j))) eqn:E.
+      * simpl. rewrite up_ren_n_swap_n.
+        apply PeanoNat.Nat.eqb_eq in E; subst. simpl. auto.
+      * simpl. destruct x; simpl.
+        ** unfold downM. rewrite (proj1 (proj2 down_ren_up_ren_commute)); auto.
+           -- apply up_ren_n_preserves_bijection; apply swap01_is_bijective.
+           -- intros; exfalso; lia.
+        ** rewrite up_ren_n_swap_not_nSn; auto. apply PeanoNat.Nat.eqb_neq in E; lia.
+  + rewrite reduce_axcut_equation_3; simpl.
+    rewrite reduce_axcut_equation_3; simpl.
+    f_equal.
+    - assert (
+        rename_process (rename_process P0 (up_ren (up_ren (up_ren_n j swap01)))) swap01 =
+        rename_process (rename_process P0 swap01) (up_ren (up_ren (up_ren_n j swap01)))
+      ).
+      {
+        erewrite (proj1 renamings_compose); auto.
+        erewrite (proj1 renamings_compose); auto.
+        intros [|[|]]; auto.
+      }
+      rewrite H2.
+      unfold down. rewrite (proj1 down_ren_up_ren_commute); auto.
+      * apply shift_preserves_bijection. apply up_ren_n_preserves_bijection; apply swap01_is_bijective.
+      * intros; exfalso; lia.
+      * apply nfv_01_swap. inversion H0; auto.
+    - inversion H; subst.
+      assert (
+        length_axcut_ctx E = length_axcut_ctx (rename_axcut_ctx E swap01)
+      ). { rewrite rename_axcut_ctx_preserves_length with (r := swap01); auto. }
+      assert (
+        well_formed_axcut_ctx 0 (rename_axcut_ctx E swap01)
+      ).
+      {
+        inversion H0; subst.
+        replace 0 with (swap01 1) by auto.
+        replace swap01 with (up_ren_n 0 swap01) by auto.
+        apply well_formedness_preserved_under_swap01; auto.
+      }
+      assert (
+        ~ (occurs_free_message (length_axcut_ctx E)
+           (rename_message M (up_ren_n (length_axcut_ctx E) swap01)))
+      ).
+      {
+        replace (length_axcut_ctx E) with
+                ((up_ren_n (length_axcut_ctx E) swap01) (S (length_axcut_ctx E)))
+          at 1
+          by apply up_ren_n_swap_Sn.
+        apply (proj1 (proj2 nfv_under_renaming)); auto.
+        apply up_ren_n_preserves_bijection; apply swap01_is_bijective.
+      }
+      replace (up_ren (up_ren_n j swap01)) with (up_ren_n (S j) swap01) by auto.
+      rewrite (IHn _ _ _ _ H2 H3 H4). f_equal.
+      * erewrite rename_axcut_ctx_compose; auto.
+        erewrite rename_axcut_ctx_compose; auto.
+        intros [|[|]]; auto.
+      * rewrite <- rename_axcut_ctx_preserves_length with (r := up_ren (up_ren_n (S j) swap01)).
+        replace (up_ren (up_ren_n (length_axcut_ctx E + S j) swap01)) with
+                (up_ren_n (S (length_axcut_ctx E + S j)) swap01) by auto.
+        replace (S (length_axcut_ctx E + S j)) with
+                (length_axcut_ctx E + S (S j)) by lia.
+        rewrite <- rename_axcut_ctx_preserves_length with (r := swap01).
+        erewrite (proj1 (proj2 renamings_compose)); auto.
+        erewrite (proj1 (proj2 renamings_compose)); auto.
+        intro x.
+        {
+          destruct (PeanoNat.Nat.eq_dec (length_axcut_ctx E) x); subst.
+          + unfold Basics.compose. rewrite up_ren_n_swap_n.
+            assert (
+              (up_ren_n (length_axcut_ctx E + S (S j)) swap01 (length_axcut_ctx E)) =
+              length_axcut_ctx E
+            ). { rewrite up_ren_n_swap_not_nSn; lia. }
+            rewrite H5. rewrite up_ren_n_swap_n.
+            rewrite up_ren_n_swap_not_nSn; lia.
+          + destruct (PeanoNat.Nat.eq_dec (S (length_axcut_ctx E)) x); subst.
+            - unfold Basics.compose. rewrite up_ren_n_swap_Sn.
+              rewrite (up_ren_n_swap_not_nSn (length_axcut_ctx E + S (S j))); try lia.
+              rewrite up_ren_n_swap_Sn. rewrite up_ren_n_swap_not_nSn; lia.
+            - unfold Basics.compose.
+              rewrite (up_ren_n_swap_not_nSn (length_axcut_ctx E) x); try lia.
+              destruct (PeanoNat.Nat.eq_dec (length_axcut_ctx E + S (S j)) x).
+              * subst. rewrite up_ren_n_swap_n.
+                rewrite up_ren_n_swap_not_nSn; lia.
+              * destruct (PeanoNat.Nat.eq_dec (S (length_axcut_ctx E + S (S j))) x).
+                ** subst. rewrite up_ren_n_swap_Sn.
+                   rewrite up_ren_n_swap_not_nSn; lia.
+                ** rewrite (up_ren_n_swap_not_nSn (length_axcut_ctx E + S (S j))); try lia.
+                   rewrite up_ren_n_swap_not_nSn; lia.
+        }
+      * unfold up. rewrite <- (proj1 ren_up_up_ren_commute).
+        ** remember (lift_process P 0 1); simpl.
+           erewrite (proj1 renamings_compose); auto.
+           erewrite (proj1 renamings_compose); auto.
+           intros [|[|]]; auto.
+        ** apply up_ren_n_preserves_bijection; apply swap01_is_bijective.
+        ** intros; exfalso; lia.
+  + rewrite reduce_axcut_equation_4; simpl.
+    rewrite reduce_axcut_equation_4; simpl.
+    f_equal.
+    - inversion H; subst.
+      assert (
+        length_axcut_ctx E = length_axcut_ctx (rename_axcut_ctx E swap01)
+      ). { rewrite rename_axcut_ctx_preserves_length with (r := swap01); auto. }
+      assert (
+        well_formed_axcut_ctx 0 (rename_axcut_ctx E swap01)
+      ).
+      {
+        inversion H0; subst.
+        replace 0 with (swap01 1) by auto.
+        replace swap01 with (up_ren_n 0 swap01) by auto.
+        apply well_formedness_preserved_under_swap01; auto.
+      }
+      assert (
+        ~ (occurs_free_message (length_axcut_ctx E)
+           (rename_message M (up_ren_n (length_axcut_ctx E) swap01)))
+      ).
+      {
+        replace (length_axcut_ctx E) with
+                ((up_ren_n (length_axcut_ctx E) swap01) (S (length_axcut_ctx E)))
+          at 1
+          by apply up_ren_n_swap_Sn.
+        apply (proj1 (proj2 nfv_under_renaming)); auto.
+        apply up_ren_n_preserves_bijection; apply swap01_is_bijective.
+      }
+      replace (up_ren (up_ren_n j swap01)) with (up_ren_n (S j) swap01) by auto.
+      rewrite (IHn _ _ _ _ H2 H3 H4). f_equal.
+      * erewrite rename_axcut_ctx_compose; auto.
+        erewrite rename_axcut_ctx_compose; auto.
+        intros [|[|]]; auto.
+      * rewrite <- rename_axcut_ctx_preserves_length with (r := up_ren (up_ren_n (S j) swap01)).
+        replace (up_ren (up_ren_n (length_axcut_ctx E + S j) swap01)) with
+                (up_ren_n (S (length_axcut_ctx E + S j)) swap01) by auto.
+        replace (S (length_axcut_ctx E + S j)) with
+                (length_axcut_ctx E + S (S j)) by lia.
+        rewrite <- rename_axcut_ctx_preserves_length with (r := swap01).
+        erewrite (proj1 (proj2 renamings_compose)); auto.
+        erewrite (proj1 (proj2 renamings_compose)); auto.
+        intro x.
+        {
+          destruct (PeanoNat.Nat.eq_dec (length_axcut_ctx E) x); subst.
+          + unfold Basics.compose. rewrite up_ren_n_swap_n.
+            assert (
+              (up_ren_n (length_axcut_ctx E + S (S j)) swap01 (length_axcut_ctx E)) =
+              length_axcut_ctx E
+            ). { rewrite up_ren_n_swap_not_nSn; lia. }
+            rewrite H5. rewrite up_ren_n_swap_n.
+            rewrite up_ren_n_swap_not_nSn; lia.
+          + destruct (PeanoNat.Nat.eq_dec (S (length_axcut_ctx E)) x); subst.
+            - unfold Basics.compose. rewrite up_ren_n_swap_Sn.
+              rewrite (up_ren_n_swap_not_nSn (length_axcut_ctx E + S (S j))); try lia.
+              rewrite up_ren_n_swap_Sn. rewrite up_ren_n_swap_not_nSn; lia.
+            - unfold Basics.compose.
+              rewrite (up_ren_n_swap_not_nSn (length_axcut_ctx E) x); try lia.
+              destruct (PeanoNat.Nat.eq_dec (length_axcut_ctx E + S (S j)) x).
+              * subst. rewrite up_ren_n_swap_n.
+                rewrite up_ren_n_swap_not_nSn; lia.
+              * destruct (PeanoNat.Nat.eq_dec (S (length_axcut_ctx E + S (S j))) x).
+                ** subst. rewrite up_ren_n_swap_Sn.
+                   rewrite up_ren_n_swap_not_nSn; lia.
+                ** rewrite (up_ren_n_swap_not_nSn (length_axcut_ctx E + S (S j))); try lia.
+                   rewrite up_ren_n_swap_not_nSn; lia.
+        }
+      * unfold up. rewrite <- (proj1 ren_up_up_ren_commute).
+        ** remember (lift_process P 0 1); simpl.
+           erewrite (proj1 renamings_compose); auto.
+           erewrite (proj1 renamings_compose); auto.
+           intros [|[|]]; auto.
+        ** apply up_ren_n_preserves_bijection; apply swap01_is_bijective.
+        ** intros; exfalso; lia.
+    - assert (
+        rename_process (rename_process P0 (up_ren (up_ren (up_ren_n j swap01)))) swap01 =
+        rename_process (rename_process P0 swap01) (up_ren (up_ren (up_ren_n j swap01)))
+      ).
+      {
+        erewrite (proj1 renamings_compose); auto.
+        erewrite (proj1 renamings_compose); auto.
+        intros [|[|]]; auto.
+      }
+      rewrite H2.
+      unfold down. rewrite (proj1 down_ren_up_ren_commute); auto.
+      * apply shift_preserves_bijection. apply up_ren_n_preserves_bijection; apply swap01_is_bijective.
+      * intros; exfalso; lia.
+      * apply nfv_01_swap. inversion H0; auto.
+Qed.
+
+Lemma up_ren_swap_over_reduce_axcut :
+  forall E M P j,
+    well_formed_axcut_ctx 0 E ->
+    ~ (occurs_free_message (length_axcut_ctx E) M) ->
+    rename_process (reduce_axcut E M P) (up_ren_n j swap01) =
+    reduce_axcut
+      (rename_axcut_ctx E (up_ren_n (S j) swap01))
+      (rename_message M (up_ren_n (length_axcut_ctx E + (S j)) swap01))
+      (rename_process P (up_ren_n (S j) swap01)).
+Proof.
+  intros. eapply up_ren_swap_over_reduce_axcut'; eauto.
+Qed.
+
+Lemma equiv_red_invariant_under_swap :
+  forall Γ P P', Γ ⊢ P :# -> P ⊵ P' -> forall j,
+    rename_process P (up_ren_n j swap01) ⊵ rename_process P' (up_ren_n j swap01).
+Proof.
+  intros.
+  generalize dependent Γ.
+  generalize dependent j.
+  induction H0; intros; try (now (simpl; econstructor)).
+  + simpl. econstructor. rewrite H.
+    unfold up. rewrite <- (proj1 ren_up_up_ren_commute).
+    - replace (up_ren (up_ren (up_ren_n j swap01))) with (up_ren_n (S (S j)) swap01) by auto.
+      rewrite ((proj1 renamings_compose) _
+        swap01
+        (up_ren_n (S (S j)) swap01)
+        (Basics.compose (up_ren_n (S (S j)) swap01) swap01)).
+      {
+        rewrite ((proj1 renamings_compose) _
+        (up_ren_n (S (S j)) swap01)
+        swap01
+        (Basics.compose (up_ren_n (S (S j)) swap01) swap01)); auto.
+      }
+      intros [|[|]]; auto.
+    - replace (up_ren (up_ren_n j swap01)) with (up_ren_n (S j) swap01) by auto.
+      apply up_ren_n_preserves_bijection. apply swap01_is_bijective.
+    - intros; exfalso; lia.
+  + simpl. econstructor. rewrite H.
+    unfold up. rewrite <- (proj1 ren_up_up_ren_commute).
+    - replace (up_ren (up_ren (up_ren_n j swap01))) with (up_ren_n (S (S j)) swap01) by auto.
+      rewrite ((proj1 renamings_compose) _
+        swap01
+        (up_ren_n (S (S j)) swap01)
+        (Basics.compose (up_ren_n (S (S j)) swap01) swap01)).
+      {
+        rewrite ((proj1 renamings_compose) _
+        (up_ren_n (S (S j)) swap01)
+        swap01
+        (Basics.compose (up_ren_n (S (S j)) swap01) swap01)); auto.
+      }
+      intros [|[|]]; auto.
+    - replace (up_ren (up_ren_n j swap01)) with (up_ren_n (S j) swap01) by auto.
+      apply up_ren_n_preserves_bijection. apply swap01_is_bijective.
+    - intros; exfalso; lia.
+  + simpl.
+    rewrite H.
+    rewrite rename_axcut_ctx_over_fill_hole.
+    - replace (up_ren (up_ren_n j swap01)) with (up_ren_n (S j) swap01) by auto.
+      rewrite H1. econstructor; eauto.
+      * replace 0 with (up_ren_n (S j) swap01 0) by auto.
+        apply well_formedness_preserved_under_swap01; auto.
+      * rewrite up_ren_n_additive.
+        apply up_ren_swap_over_reduce_axcut; auto.
+        inversion H2; subst.
+        replace (length_axcut_ctx E) with (length_axcut_ctx E + 0) by lia.
+        eapply nfv_well_typed_fill_hole; eauto.
+    - replace (up_ren (up_ren_n j swap01)) with (up_ren_n (S j) swap01) by auto.
+      apply up_ren_n_preserves_bijection; apply swap01_is_bijective.
+  + simpl.
+    rewrite H.
+    rewrite rename_axcut_ctx_over_fill_hole.
+    - replace (up_ren (up_ren_n j swap01)) with (up_ren_n (S j) swap01) by auto.
+      rewrite H1. eapply rp_ax_cut_r; eauto.
+      * replace 0 with (up_ren_n (S j) swap01 0) by auto.
+        apply well_formedness_preserved_under_swap01; auto.
+      * rewrite up_ren_n_additive.
+        apply up_ren_swap_over_reduce_axcut; auto.
+        inversion H2; subst.
+        replace (length_axcut_ctx E) with (length_axcut_ctx E + 0) by lia.
+        eapply nfv_well_typed_fill_hole; eauto.
+    - replace (up_ren (up_ren_n j swap01)) with (up_ren_n (S j) swap01) by auto.
+      apply up_ren_n_preserves_bijection; apply swap01_is_bijective.
+  + simpl.
+    rewrite (proj1 up_ren_swap_over_subst). simpl.
+    rewrite ((proj1 subst_extensional) _ _
+             ((prefix (rename_statement s (up_ren_n j swap01))) ⋅ id_subst)).
+    - econstructor.
+    - intros. destruct x; auto. simpl.
+      unfold swap_subst.
+      destruct (Nat.eqb (S x) (S j)) eqn:E1; simpl.
+      * apply PeanoNat.Nat.eqb_eq in E1; inversion E1; subst.
+        rewrite up_ren_n_swap_Sn. auto.
+      * destruct (Nat.eqb x (S j)) eqn:E2; simpl.
+        ** apply PeanoNat.Nat.eqb_eq in E2; subst.
+            rewrite up_ren_n_swap_n; auto.
+        ** apply PeanoNat.Nat.eqb_neq in E1, E2.
+           assert (x <> j) by lia.
+           rewrite up_ren_n_swap_not_nSn; auto.
+  + simpl. apply rp_cong_cut_l.
+    replace (up_ren (up_ren_n j swap01)) with (up_ren_n (S j) swap01) by auto.
+    inversion H; subst.
+    eapply IHequiv_reduces; eauto.
+  + simpl. apply rp_cong_cut_r.
+    replace (up_ren (up_ren_n j swap01)) with (up_ren_n (S j) swap01) by auto.
+    inversion H; subst.
+    eapply IHequiv_reduces; eauto.
+  + simpl. apply rp_cong_seq.
+    replace (up_ren (up_ren_n j swap01)) with (up_ren_n (S j) swap01) by auto.
+    inversion H; subst.
+    eapply IHequiv_reduces; eauto.
+Qed.
+
+(* ⊵ is invariant under lifting ***********************************************)
+Definition lift_subst_at_n (σ : substitution) (n : nat) : substitution :=
+  fun x => if (Nat.eqb x (S n)) then (future n) else
+            if (Nat.ltb (S n) x) then (lift_message (σ (Nat.pred x)) n 1)
+             else (lift_message (σ x) n 1).
+
+Lemma up_subst_over_lift_subst :
+  forall σ n x,
+    up_subst (lift_subst_at_n σ n) x = lift_subst_at_n (up_subst σ) (S n) x.
+Proof.
+  intros.
+  destruct x; auto; simpl.
+  unfold lift_subst_at_n.
+  destruct (Nat.eqb x (S n)) eqn:E1.
+  + apply PeanoNat.Nat.eqb_eq in E1. assert (S x = S (S n)) by lia.
+    apply PeanoNat.Nat.eqb_eq in H; rewrite H.
+    simpl. reflexivity.
+  + destruct (Nat.ltb (S n) x) eqn:E2.
+    - apply PeanoNat.Nat.ltb_lt in E2.
+      assert (S (S n) < (S x)) by lia. apply PeanoNat.Nat.ltb_lt in H; rewrite H.
+      assert (S x <> S (S n)) by lia. apply PeanoNat.Nat.eqb_neq in H0; rewrite H0.
+      apply PeanoNat.Nat.ltb_lt in H; apply PeanoNat.Nat.eqb_neq in H0.
+      destruct x; try (exfalso; lia). simpl.
+      unfold upM. rewrite (proj1 (proj2 lift_k_lift_Sj_lt_commute)); auto. lia.
+    - apply PeanoNat.Nat.eqb_neq in E1. assert (S x <> S (S n)) by lia.
+      apply PeanoNat.Nat.eqb_neq in H; rewrite H.
+      apply PeanoNat.Nat.ltb_nlt in E2. assert (~ (S (S n)) < S x) by lia.
+      apply PeanoNat.Nat.ltb_nlt in H0; rewrite H0; simpl.
+      unfold upM. rewrite (proj1 (proj2 lift_k_lift_Sj_lt_commute)); auto. lia.
+Qed.
+
+Lemma up_subst_over_lift_subst2 :
+  forall σ n x,
+    up_subst (up_subst (lift_subst_at_n σ n)) x
+      = lift_subst_at_n (up_subst (up_subst σ)) (S (S n)) x.
+Proof.
+  destruct x; auto; simpl. destruct x; auto; simpl.
+  unfold lift_subst_at_n.
+    destruct (Nat.eqb x (S n)) eqn:E1.
+  + apply PeanoNat.Nat.eqb_eq in E1. assert (S (S x) = S (S (S n))) by lia.
+    apply PeanoNat.Nat.eqb_eq in H; rewrite H.
+    simpl. reflexivity.
+  + destruct (Nat.ltb (S n) x) eqn:E2.
+    - apply PeanoNat.Nat.ltb_lt in E2.
+      assert (S (S (S n)) < (S (S x))) by lia. apply PeanoNat.Nat.ltb_lt in H; rewrite H.
+      assert (S (S x) <> S (S (S n))) by lia. apply PeanoNat.Nat.eqb_neq in H0; rewrite H0.
+      apply PeanoNat.Nat.ltb_lt in H; apply PeanoNat.Nat.eqb_neq in H0.
+      destruct x; try (exfalso; lia). simpl.
+      unfold upM. rewrite (proj1 (proj2 lift_k_lift_Sj_lt_commute)); auto; try lia.
+      rewrite (proj1 (proj2 lift_k_lift_Sj_lt_commute)); auto; try lia.
+    - apply PeanoNat.Nat.eqb_neq in E1. assert (S (S x) <> S (S (S n))) by lia.
+      apply PeanoNat.Nat.eqb_neq in H; rewrite H.
+      apply PeanoNat.Nat.ltb_nlt in E2. assert (~ (S (S (S n))) < S (S x)) by lia.
+      apply PeanoNat.Nat.ltb_nlt in H0; rewrite H0; simpl.
+      unfold upM. rewrite (proj1 (proj2 lift_k_lift_Sj_lt_commute)); auto; try lia.
+      rewrite (proj1 (proj2 lift_k_lift_Sj_lt_commute)); auto; try lia.
+Qed.
+
+Lemma lift_over_subst :
+  (
+    forall P, forall σ j,
+      lift_process (subst_process P σ) j 1 =
+      subst_process (lift_process P (S j) 1) (lift_subst_at_n σ j)
+  ) /\
+  (
+    forall M, forall σ j,
+      lift_message (subst_message M σ) j 1 =
+      subst_message (lift_message M (S j) 1) (lift_subst_at_n σ j)
+  ) /\
+  (
+    forall s, forall σ j,
+      lift_statement (subst_statement s σ) j 1 =
+      subst_statement (lift_statement s (S j) 1) (lift_subst_at_n σ j)
+  ).
+Proof.
+  apply syntax_ind; intros; simpl;
+  try (now (try rewrite H; try rewrite H0; auto));
+  try repeat rewrite ((proj1 subst_extensional) _
+              (up_subst (lift_subst_at_n σ j))
+              (lift_subst_at_n (up_subst σ) (S j))
+              (up_subst_over_lift_subst _ _));
+  try rewrite H; try rewrite H0; auto.
+  + unfold lift_subst_at_n, relocate.
+    destruct (Nat.leb (S j) n) eqn:E1; simpl.
+    - destruct (Nat.eqb n j) eqn:E2.
+      * exfalso.
+        apply PeanoNat.Nat.leb_le in E1.
+        apply PeanoNat.Nat.eqb_eq in E2.
+        lia.
+      * apply PeanoNat.Nat.leb_le in E1.
+        apply PeanoNat.Nat.eqb_neq in E2.
+        assert (S j < S n) by lia. apply PeanoNat.Nat.ltb_lt in H; rewrite H.
+        reflexivity.
+    - destruct (Nat.eqb n (S j)) eqn:E2.
+      * exfalso.
+        apply PeanoNat.Nat.leb_nle in E1.
+        apply PeanoNat.Nat.eqb_eq in E2.
+        lia.
+      * apply PeanoNat.Nat.leb_nle in E1.
+        apply PeanoNat.Nat.eqb_neq in E2.
+        assert (~ (S j) < n) by lia. apply PeanoNat.Nat.ltb_nlt in H; rewrite H.
+        reflexivity.
+  + f_equal. apply subst_extensional. intro.
+    rewrite up_subst_over_lift_subst2; auto.
+Qed.
+
+Lemma lift_ctx_at_k_rename_ctx_id_after_k_commute :
+  forall E k r,
+    bijective r -> (forall j, k <= j -> r j = j) ->
+      lift_ctx (rename_axcut_ctx E r) k 1
+        = rename_axcut_ctx (lift_ctx E k 1) r.
+Proof.
+  intro E. induction E; intros; simpl.
+  + f_equal.
+    unfold relocate.
+    destruct (Nat.leb k n) eqn:E.
+    - apply PeanoNat.Nat.leb_le in E. rewrite (H0 _ E).
+      apply PeanoNat.Nat.leb_le in E. rewrite E. simpl.
+      apply PeanoNat.Nat.leb_le in E.
+      rewrite H0; lia.
+    - apply PeanoNat.Nat.leb_nle in E.
+      assert ( ~ k <= (r n) ).
+      {
+        intro Hle. destruct H.
+        replace n with (g (r n)) in E by (rewrite c; auto).
+        rewrite <- (H0 _ Hle) in E.
+        rewrite c in E. congruence.
+      }
+      apply PeanoNat.Nat.leb_nle in H1; rewrite H1; auto.
+  + f_equal.
+    unfold relocate.
+    destruct (Nat.leb k n) eqn:E.
+    - apply PeanoNat.Nat.leb_le in E. rewrite (H0 _ E).
+      apply PeanoNat.Nat.leb_le in E. rewrite E. simpl.
+      apply PeanoNat.Nat.leb_le in E.
+      rewrite H0; lia.
+    - apply PeanoNat.Nat.leb_nle in E.
+      assert ( ~ k <= (r n) ).
+      {
+        intro Hle. destruct H.
+        replace n with (g (r n)) in E by (rewrite c; auto).
+        rewrite <- (H0 _ Hle) in E.
+        rewrite c in E. congruence.
+      }
+      apply PeanoNat.Nat.leb_nle in H1; rewrite H1; auto.
+  + f_equal.
+    - rewrite (proj1 lift_at_k_rename_id_after_k_commute); auto.
+      apply shift_preserves_bijection; auto.
+      intros. destruct j; auto. assert (k <= j) by lia.
+      simpl. rewrite (H0 _ H2). reflexivity.
+    - rewrite IHE; auto.
+      apply shift_preserves_bijection; auto.
+      intros. destruct j; auto. assert (k <= j) by lia.
+      simpl. rewrite (H0 _ H2). reflexivity.
+  + f_equal.
+    - rewrite IHE; auto.
+      apply shift_preserves_bijection; auto.
+      intros. destruct j; auto. assert (k <= j) by lia.
+      simpl. rewrite (H0 _ H2). reflexivity.
+    - rewrite (proj1 lift_at_k_rename_id_after_k_commute); auto.
+      apply shift_preserves_bijection; auto.
+      intros. destruct j; auto. assert (k <= j) by lia.
+      simpl. rewrite (H0 _ H2). reflexivity.
+Qed.
+
+Lemma lift_after_down_lt_commute_nfv :
+  (forall P,
+    forall k1 k2, k2 <= k1 ->
+      ~ (k2 ∈ P) ->
+      lift_process (down1_process P k2) k1 1
+        = down1_process (lift_process P (S k1) 1) k2) /\
+  (forall M,
+    forall k1 k2, k2 <= k1 ->
+      ~ (occurs_free_message k2 M) ->
+      lift_message (down1_message M k2) k1 1
+        = down1_message (lift_message M (S k1) 1) k2) /\
+  (forall s,
+    forall k1 k2, k2 <= k1 ->
+      ~ (occurs_free_statement k2 s) ->
+      lift_statement (down1_statement s k2) k1 1
+        = down1_statement (lift_statement s (S k1) 1) k2).
+Proof.
+  apply syntax_ind; intros; simpl; auto.
+    try (now (rewrite (H (S k1) (S k2)); try lia; try free_var_econstructor; eauto));
+    try (now (rewrite (H (S k1) (S k2)); try lia; rewrite (H0 (S k1) (S k2)); try lia; auto)).
+  + rewrite H; auto; try rewrite H0; auto; intro Hfv; apply H2; free_var_econstructor; eauto.
+  + rewrite (H (S k1) (S k2)); try lia; try rewrite (H0 (S k1) (S k2)); try lia; auto;
+    intro Hfv; apply H2; free_var_econstructor; eauto.
+  + rewrite (H (S k1) (S k2)); auto; try rewrite (H0 k1 k2); try lia; auto;
+    intro Hfv; apply H2; free_var_econstructor; eauto.
+  + unfold relocate.
+    destruct (Nat.leb (S k1) n) eqn:E.
+    - simpl. apply PeanoNat.Nat.leb_le in E.
+      assert (k2 < n) by lia. apply PeanoNat.Nat.ltb_lt in H1.
+      assert (k2 < S n) by lia. apply PeanoNat.Nat.ltb_lt in H2.
+      rewrite H1, H2. destruct n; try (exfalso; lia). simpl.
+      unfold relocate. assert (k1 <= n) by lia.
+      apply PeanoNat.Nat.leb_le in H3. rewrite H3; reflexivity.
+    - apply PeanoNat.Nat.leb_nle in E.
+      assert (n <= k1) by lia.
+      destruct (Nat.ltb k2 n) eqn:E1.
+      * simpl. unfold relocate. destruct (PeanoNat.Nat.eq_dec k2 n). { subst; exfalso; apply H0; econstructor. }
+        assert (~ (k1 <= (Nat.pred n))) by lia.
+        apply PeanoNat.Nat.leb_nle in H2. rewrite H2. reflexivity.
+      * simpl. unfold relocate.
+        apply PeanoNat.Nat.ltb_nlt in E1.
+        destruct (PeanoNat.Nat.eq_dec n k1).
+        ++ destruct (PeanoNat.Nat.eq_dec k2 n). { subst; exfalso; apply H0; econstructor. }
+           exfalso. lia.
+        ++ assert (~ (k1 <= n)) by lia. apply PeanoNat.Nat.leb_nle in H2. rewrite H2. reflexivity.
+  + rewrite H; auto; try lia; intro Hfv; apply H1; free_var_econstructor; eauto.
+  + rewrite H; auto; try lia; intro Hfv; apply H1; free_var_econstructor; eauto.
+  + rewrite H; auto; try lia; intro Hfv; apply H1; free_var_econstructor; eauto.
+  + rewrite (H (S k1) (S k2)); try lia; try rewrite (H0 (S k1) (S k2)); try lia; auto;
+    intro Hfv; apply H2; free_var_econstructor; eauto.
+  + rewrite (H (S k1) (S k2)); try lia; try rewrite (H0 (S k1) (S k2)); try lia; auto;
+    intro Hfv; apply H2; free_var_econstructor; eauto.
+  + rewrite (H (S (S k1)) (S (S k2))); try lia; try rewrite (H0 (S k1) (S k2)); try lia; auto;
+    intro Hfv; apply H1; free_var_econstructor; eauto.
+  + rewrite H; auto; try lia; intro Hfv; apply H1; free_var_econstructor; eauto.
+Qed.
+
+Lemma lift_over_reduce_axcut' :
+  forall n E M P j,
+    n = length_axcut_ctx E ->
+    well_formed_axcut_ctx 0 E ->
+    ~ (occurs_free_message (length_axcut_ctx E) M) ->
+    lift_process (reduce_axcut E M P) j 1 =
+    reduce_axcut
+      (lift_ctx E (S j) 1)
+      (lift_message M (length_axcut_ctx E + S j) 1)
+      (lift_process P (S j) 1).
+Proof.
+  intro n.
+  induction n; intros;
+  destruct E; simpl in H; try congruence; simpl.
+  + rewrite reduce_axcut_equation_1.
+    unfold relocate. destruct (Nat.leb (S j) n) eqn:E; simpl.
+    - rewrite reduce_axcut_equation_1.
+      rewrite (proj1 lift_over_subst). erewrite (proj1 subst_extensional); eauto.
+      apply PeanoNat.Nat.leb_le in E.
+      intros.
+      unfold lift_subst_at_n. destruct (Nat.eqb x (S j)) eqn:E1.
+      * apply PeanoNat.Nat.eqb_eq in E1; subst; auto.
+      * apply PeanoNat.Nat.eqb_neq in E1.
+        destruct (Nat.ltb (S j) x) eqn:E2.
+        ** apply PeanoNat.Nat.ltb_lt in E2. destruct x; try (exfalso; lia).
+           simpl. destruct x; try (exfalso; lia). simpl.
+           unfold relocate. assert (j <= x) by lia. apply PeanoNat.Nat.leb_le in H2.
+           rewrite H2; auto.
+        ** apply PeanoNat.Nat.ltb_nlt in E2. destruct x; simpl.
+          *** unfold downM.
+              rewrite (proj1 (proj2 lift_after_down_lt_commute_nfv)); auto.
+              lia.
+          *** unfold relocate. assert (~ (j <= x)) by lia. apply PeanoNat.Nat.leb_nle in H2.
+              rewrite H2. auto.
+    - rewrite reduce_axcut_equation_1.
+      rewrite (proj1 lift_over_subst). erewrite (proj1 subst_extensional); eauto.
+      apply PeanoNat.Nat.leb_nle in E.
+      intros.
+      unfold lift_subst_at_n. destruct (Nat.eqb x (S j)) eqn:E1.
+      * apply PeanoNat.Nat.eqb_eq in E1; subst; auto.
+      * apply PeanoNat.Nat.eqb_neq in E1.
+        destruct (Nat.ltb (S j) x) eqn:E2.
+        ** apply PeanoNat.Nat.ltb_lt in E2. destruct x; try (exfalso; lia).
+           simpl. destruct x; try (exfalso; lia). simpl.
+           unfold relocate. assert (j <= x) by lia. apply PeanoNat.Nat.leb_le in H2.
+           rewrite H2; auto.
+        ** apply PeanoNat.Nat.ltb_nlt in E2. destruct x; simpl.
+          *** unfold downM.
+              rewrite (proj1 (proj2 lift_after_down_lt_commute_nfv)); auto.
+              lia.
+          *** unfold relocate. assert (~ (j <= x)) by lia. apply PeanoNat.Nat.leb_nle in H2.
+              rewrite H2. auto.
+  + rewrite reduce_axcut_equation_2.
+    unfold relocate. destruct (Nat.leb (S j) n) eqn:E; simpl.
+    - rewrite reduce_axcut_equation_2.
+      rewrite (proj1 lift_over_subst). erewrite (proj1 subst_extensional); eauto.
+      apply PeanoNat.Nat.leb_le in E.
+      intros.
+      unfold lift_subst_at_n. destruct (Nat.eqb x (S j)) eqn:E1.
+      * apply PeanoNat.Nat.eqb_eq in E1; subst; auto.
+      * apply PeanoNat.Nat.eqb_neq in E1.
+        destruct (Nat.ltb (S j) x) eqn:E2.
+        ** apply PeanoNat.Nat.ltb_lt in E2. destruct x; try (exfalso; lia).
+           simpl. destruct x; try (exfalso; lia). simpl.
+           unfold relocate. assert (j <= x) by lia. apply PeanoNat.Nat.leb_le in H2.
+           rewrite H2; auto.
+        ** apply PeanoNat.Nat.ltb_nlt in E2. destruct x; simpl.
+          *** unfold downM.
+              rewrite (proj1 (proj2 lift_after_down_lt_commute_nfv)); auto.
+              lia.
+          *** unfold relocate. assert (~ (j <= x)) by lia. apply PeanoNat.Nat.leb_nle in H2.
+              rewrite H2. auto.
+    - rewrite reduce_axcut_equation_2.
+      rewrite (proj1 lift_over_subst). erewrite (proj1 subst_extensional); eauto.
+      apply PeanoNat.Nat.leb_nle in E.
+      intros.
+      unfold lift_subst_at_n. destruct (Nat.eqb x (S j)) eqn:E1.
+      * apply PeanoNat.Nat.eqb_eq in E1; subst; auto.
+      * apply PeanoNat.Nat.eqb_neq in E1.
+        destruct (Nat.ltb (S j) x) eqn:E2.
+        ** apply PeanoNat.Nat.ltb_lt in E2. destruct x; try (exfalso; lia).
+           simpl. destruct x; try (exfalso; lia). simpl.
+           unfold relocate. assert (j <= x) by lia. apply PeanoNat.Nat.leb_le in H2.
+           rewrite H2; auto.
+        ** apply PeanoNat.Nat.ltb_nlt in E2. destruct x; simpl.
+          *** unfold downM.
+              rewrite (proj1 (proj2 lift_after_down_lt_commute_nfv)); auto.
+              lia.
+          *** unfold relocate. assert (~ (j <= x)) by lia. apply PeanoNat.Nat.leb_nle in H2.
+              rewrite H2. auto.
+  + rewrite reduce_axcut_equation_3; simpl.
+    rewrite reduce_axcut_equation_3; simpl.
+    f_equal.
+    - unfold down. rewrite (proj1 lift_after_down_lt_commute); try lia.
+      f_equal. rewrite (proj1 lift_at_k_rename_id_after_k_commute); auto.
+      apply swap01_is_bijective. intros [|[|]] ?; try (exfalso; lia); auto.
+    - inversion H; subst.
+      assert (
+        length_axcut_ctx E = length_axcut_ctx (rename_axcut_ctx E swap01)
+      ). { rewrite rename_axcut_ctx_preserves_length with (r := swap01); auto. }
+      assert (
+        well_formed_axcut_ctx 0 (rename_axcut_ctx E swap01)
+      ).
+      {
+        inversion H0; subst.
+        replace 0 with (swap01 1) by auto.
+        replace swap01 with (up_ren_n 0 swap01) by auto.
+        apply well_formedness_preserved_under_swap01; auto.
+      }
+      assert (
+        ~ (occurs_free_message (length_axcut_ctx E)
+           (rename_message M (up_ren_n (length_axcut_ctx E) swap01)))
+      ).
+      {
+        replace (length_axcut_ctx E) with
+                ((up_ren_n (length_axcut_ctx E) swap01) (S (length_axcut_ctx E)))
+          at 1
+          by apply up_ren_n_swap_Sn.
+        apply (proj1 (proj2 nfv_under_renaming)); auto.
+        apply up_ren_n_preserves_bijection; apply swap01_is_bijective.
+      }
+      rewrite H2.
+      rewrite H2 in H4.
+      rewrite (IHn _ _ _  _  H2 H3 H4). f_equal.
+      * rewrite lift_ctx_at_k_rename_ctx_id_after_k_commute; auto.
+        apply swap01_is_bijective. intros [|[|]] ?; try (exfalso; lia); auto.
+      * rewrite <- rename_axcut_ctx_preserves_length with (r := swap01).
+        rewrite lift_ctx_preserves_length.
+        replace (S (length_axcut_ctx E + S j))
+           with (length_axcut_ctx E + S (S j))
+             by lia.
+        rewrite (proj1 (proj2 lift_at_k_rename_id_after_k_commute)); auto.
+        apply up_ren_n_preserves_bijection; apply swap01_is_bijective.
+        intros. apply up_ren_n_swap_not_nSn; lia.
+      * unfold up.
+        rewrite (proj1 lift_at_k_rename_id_after_k_commute).
+        ** f_equal. rewrite (proj1 lift_k_lift_Sj_lt_commute); auto. lia.
+        ** apply swap01_is_bijective.
+        ** intros [|[|]] ?; try (exfalso; lia); auto.
+  + rewrite reduce_axcut_equation_4; simpl.
+    rewrite reduce_axcut_equation_4; simpl.
+    f_equal.
+    - inversion H; subst.
+      assert (
+        length_axcut_ctx E = length_axcut_ctx (rename_axcut_ctx E swap01)
+      ). { rewrite rename_axcut_ctx_preserves_length with (r := swap01); auto. }
+      assert (
+        well_formed_axcut_ctx 0 (rename_axcut_ctx E swap01)
+      ).
+      {
+        inversion H0; subst.
+        replace 0 with (swap01 1) by auto.
+        replace swap01 with (up_ren_n 0 swap01) by auto.
+        apply well_formedness_preserved_under_swap01; auto.
+      }
+      assert (
+        ~ (occurs_free_message (length_axcut_ctx E)
+           (rename_message M (up_ren_n (length_axcut_ctx E) swap01)))
+      ).
+      {
+        replace (length_axcut_ctx E) with
+                ((up_ren_n (length_axcut_ctx E) swap01) (S (length_axcut_ctx E)))
+          at 1
+          by apply up_ren_n_swap_Sn.
+        apply (proj1 (proj2 nfv_under_renaming)); auto.
+        apply up_ren_n_preserves_bijection; apply swap01_is_bijective.
+      }
+      rewrite H2.
+      rewrite H2 in H4.
+      rewrite (IHn _ _ _  _  H2 H3 H4). f_equal.
+      * rewrite lift_ctx_at_k_rename_ctx_id_after_k_commute; auto.
+        apply swap01_is_bijective. intros [|[|]] ?; try (exfalso; lia); auto.
+      * rewrite <- rename_axcut_ctx_preserves_length with (r := swap01).
+        rewrite lift_ctx_preserves_length.
+        replace (S (length_axcut_ctx E + S j))
+           with (length_axcut_ctx E + S (S j))
+             by lia.
+        rewrite (proj1 (proj2 lift_at_k_rename_id_after_k_commute)); auto.
+        apply up_ren_n_preserves_bijection; apply swap01_is_bijective.
+        intros. apply up_ren_n_swap_not_nSn; lia.
+      * unfold up.
+        rewrite (proj1 lift_at_k_rename_id_after_k_commute).
+        ** f_equal. rewrite (proj1 lift_k_lift_Sj_lt_commute); auto. lia.
+        ** apply swap01_is_bijective.
+        ** intros [|[|]] ?; try (exfalso; lia); auto.
+    - unfold down. rewrite (proj1 lift_after_down_lt_commute); try lia.
+      f_equal. rewrite (proj1 lift_at_k_rename_id_after_k_commute); auto.
+      apply swap01_is_bijective. intros [|[|]] ?; try (exfalso; lia); auto.
+Qed.
+
+Lemma lift_over_reduce_axcut :
+  forall E M P j,
+    well_formed_axcut_ctx 0 E ->
+    ~ (occurs_free_message (length_axcut_ctx E) M) ->
+    lift_process (reduce_axcut E M P) j 1 =
+    reduce_axcut
+      (lift_ctx E (S j) 1)
+      (lift_message M (length_axcut_ctx E + S j) 1)
+      (lift_process P (S j) 1).
+Proof.
+  intros. eapply lift_over_reduce_axcut'; eauto.
+Qed.
+
+Lemma equiv_red_invariant_under_up :
+  forall Γ P P', Γ ⊢ P :# -> P ⊵ P' ->
+    forall j, lift_process P j 1 ⊵ lift_process P' j 1.
+Proof.
+  intros.
+  generalize dependent Γ.
+  generalize dependent j.
+  induction H0; intros; simpl; try (now econstructor).
+  + econstructor. subst.
+    unfold up. rewrite (proj1 lift_at_k_rename_id_after_k_commute).
+    - rewrite (proj1 lift_k_lift_Sj_lt_commute); auto. lia.
+    - apply swap01_is_bijective.
+    - intros [|[|]] ?; auto; try (exfalso; lia).
+  + econstructor. subst.
+    unfold up. rewrite (proj1 lift_at_k_rename_id_after_k_commute).
+    - rewrite (proj1 lift_k_lift_Sj_lt_commute); auto. lia.
+    - apply swap01_is_bijective.
+    - intros [|[|]] ?; auto; try (exfalso; lia).
+  + rewrite H, H1.
+    rewrite up_ctx_over_fill_hole.
+    assert (
+      lift_process (reduce_axcut E M P) j 1 =
+      reduce_axcut
+        (lift_ctx E (S j) 1)
+        (lift_message M (length_axcut_ctx E + S j) 1)
+        (lift_process P (S j) 1)
+    ).
+    {
+      apply lift_over_reduce_axcut; auto.
+      inversion H2; subst.
+      replace (length_axcut_ctx E) with (length_axcut_ctx E + 0) by lia.
+      eapply nfv_well_typed_fill_hole; eauto.
+    }
+    rewrite H3. econstructor; eauto.
+    apply upE_preserves_well_formedness2; auto. lia.
+  + rewrite H, H1.
+    rewrite up_ctx_over_fill_hole.
+    assert (
+      lift_process (reduce_axcut E M P) j 1 =
+      reduce_axcut
+        (lift_ctx E (S j) 1)
+        (lift_message M (length_axcut_ctx E + S j) 1)
+        (lift_process P (S j) 1)
+    ).
+    {
+      apply lift_over_reduce_axcut; auto.
+      inversion H2; subst.
+      replace (length_axcut_ctx E) with (length_axcut_ctx E + 0) by lia.
+      eapply nfv_well_typed_fill_hole; eauto.
+    }
+    rewrite H3. eapply rp_ax_cut_r; eauto.
+    apply upE_preserves_well_formedness2; auto. lia.
+  + rewrite (proj1 lift_over_subst).
+    erewrite (proj1 subst_extensional).
+    - econstructor.
+    - intros [|]; auto; simpl.
+      unfold lift_subst_at_n.
+      destruct (Nat.eqb (S n) (S j)) eqn:E1.
+      * apply PeanoNat.Nat.eqb_eq in E1; inversion E1; auto.
+      * destruct (PeanoNat.Nat.ltb (S j) (S n)) eqn:E2.
+        ** simpl. apply PeanoNat.Nat.ltb_lt in E2. destruct n; try (exfalso; lia).
+           simpl. unfold relocate. assert (j <= n) by lia. apply PeanoNat.Nat.leb_le in H0.
+           rewrite H0. auto.
+        ** simpl. unfold relocate.
+           apply PeanoNat.Nat.ltb_nlt in E2. apply PeanoNat.Nat.eqb_neq in E1.
+           assert (~ (j <= n)) by lia. apply PeanoNat.Nat.leb_nle in H0.
+           rewrite H0. auto.
+  + apply rp_cong_cut_l. inversion H; subst.
+    eapply IHequiv_reduces; eauto.
+  + apply rp_cong_cut_r. inversion H; subst.
+    eapply IHequiv_reduces; eauto.
+  + apply rp_cong_seq. inversion H; subst.
+    eapply IHequiv_reduces; eauto.
 Qed.
